coq-SystemRF-3.0/Bidirectional/SynthWFFT.v
@@ -1,0 +1,119 @@
+Require Import SystemRF.BasicDefinitions. 
+Require Import SystemRF.Names.
+Require Import SystemRF.SystemFWellFormedness.
+Require Import Denotations.Denotations.
+
+From Equations Require Import Equations.
+
+Require Import ZArith.
+
+Fixpoint fdepth (t : ftype) : nat :=
+    match t with
+    | (FTBasic b)    => 0
+    | (FTFunc tx t') => 1 + max (fdepth tx) (fdepth t')
+    | (FTPoly k t')  => 1 + fdepth t'
+    | (FTList t')    => 1 + fdepth t'
+    end.
+
+Lemma fdepth_openFT_at : forall (j:index) (a:vname) (t:ftype),
+    fdepth (openFT_at j a t) = fdepth t.
+Proof. intros j a t; revert j; induction t; intros;
+  simpl; try destruct b; try destruct (Nat.eqb j i); 
+  reflexivity || f_equal; apply IHt || f_equal;
+  try apply IHt1; try apply IHt2; apply H. Qed.
+
+Lemma fdepth_unbindFT : forall (a:vname) (t:ftype),
+    fdepth (unbindFT a t) = fdepth t.
+Proof. intros; apply fdepth_openFT_at; assumption. Qed.
+
+(*** we need a stack env for BTV deBruijn's and their kinds ***)
+
+(*----------------------------------------------------------------------------
+  --- | AUTOMATED INFERENCE of SYSTEM F WELL-FORMEDNESS JUDGMENTS
+  --------------------------------------------------------------------------*)
+
+Equations isWFFT (g:fenv) (t:ftype) (k:kind) : Prop 
+  by wf (fdepth t) :=
+isWFFT g (FTBasic b) k := 
+    match b with
+    | TBool    => True
+    | TInt     => True
+    | (BTV a)  => False
+    | (FTV a)  => (tv_bound_inF a Base g) \/ 
+                    (tv_bound_inF a Star g /\ k = Star)
+    end;
+isWFFT g (FTFunc t_x t) k := 
+    k = Star /\ isWFFT g t_x Star  /\ isWFFT g t   Star;
+isWFFT g (FTPoly k'  t) k := 
+    let a' := fresh_varF nil g
+    in  k = Star /\ isWFFT (FConsT a' k' g) (unbindFT a' t) Star;
+isWFFT g (FTList t) k     := 
+    k = Star /\ isWFFT g t   Star.
+  Obligation 1. (* fdepth t_x "<" fdepth t *)
+    pose proof Nat.le_max_l (fdepth  t_x) (fdepth  t) as Hd.
+    apply Nat.lt_succ_r; apply Hd.
+  Defined.
+  Obligation 2. (* fdepth t' "<" fdepth t *)
+    pose proof Nat.le_max_r (fdepth  t_x) (fdepth  t) as Hd.
+    apply Nat.lt_succ_r; apply Hd.
+  Defined.
+  Obligation 3.
+    rewrite fdepth_unbindFT; apply Nat.lt_succ_r; trivial.
+  Defined.
+
+Example isWFFT_one : isWFFT FEmpty (FTList (FTBasic TInt)) Star.
+Proof. funelim (isWFFT FEmpty (FTList (FTBasic TInt)) Star);
+  (*unfold not;*) split; intros;
+  (discriminate || contradiction || constructor). Qed.
+
+Example isWFFT_two : isWFFT FEmpty (FTPoly Base (FTBasic (BTV 0))) Star.
+Proof. funelim (isWFFT FEmpty (FTPoly Base (FTBasic (BTV 0))) Star);
+  (*unfold not;*) split; intros;
+  (discriminate || contradiction || constructor);
+  simpl; auto. Qed.  
+
+Lemma makeWFFT : forall (n:nat) (g:fenv) (t:ftype) (k:kind),
+    fdepth t <= n   -> isWFFT g t k -> WFFT g t k.
+Proof. intros n; induction n.
+  - (* Base *) intros;
+    assert (fdepth t = 0) by auto with *.
+    destruct t; simpl in H1; try discriminate.
+    destruct b; rewrite isWFFT_equation_1 in H0;
+    try contradiction; destruct k;
+    try destruct H0; 
+    try destruct H0; try discriminate;
+    try (apply WFFTFV; apply H0);
+    try apply WFFTKind;
+    try apply WFFTFV; try apply WFFTBasic;
+    simpl; trivial.
+  - (* Inductive *) intros.
+    destruct t eqn:T;
+    (* avoid proving base case again *)
+    try (assert (fdepth t <= n) as Hbase
+          by (rewrite T; simpl; auto with *);
+         apply IHn; subst t; trivial);
+    simpl in H; apply Nat.succ_le_mono in H.
+    * (* FTFunc t1 t2 *)
+      rewrite isWFFT_equation_2 in H0;
+      destruct H0; destruct H1; subst k.
+      apply WFFTFunc with Star Star; 
+      apply IHn; try apply Nat.le_trans 
+        with (Init.Nat.max (fdepth f1) (fdepth f2));
+      try apply Nat.le_max_l;
+      try apply Nat.le_max_r; trivial.
+    * (* FTPoly k0 f *)
+      rewrite isWFFT_equation_3 in H0;
+      destruct H0; subst k;
+      apply WFFTPoly with Star (bindsF g);
+      intros; apply IHn;
+      
+      try rewrite fdepth_unbindFT; trivial. 
+    * (* FTList f *) 
+      rewrite isWFFT_equation_4 in H0; destruct H0; subst k.
+      apply WFFTList with Star; 
+      apply IHn; trivial.
+    
+
+Theorem checkWFFT : forall (g:fenv) (t:ftype) (k:kind),
+    isWFFT g t k -> WFFT g t k.
+Proof. intros. apply makeWFFT with (fdepth t); trivial. Qed.
