coq-SystemRF-3.0/SystemRF/LemmasLists.v
@@ -1,0 +1,477 @@
+Require Import SystemRF.BasicDefinitions.
+Require Import SystemRF.Names.
+Require Import SystemRF.LocalClosure.
+Require Import SystemRF.Semantics.
+Require Import SystemRF.SystemFTyping.
+Require Import SystemRF.BasicPropsSubstitution.
+Require Import SystemRF.BasicPropsEnvironments.
+Require Import SystemRF.PrimitivesFTyping.
+Require Import SystemRF.WellFormedness.
+Require Import SystemRF.BasicPropsWellFormedness.
+Require Import SystemRF.SystemFLemmasWellFormedness.
+Require Import SystemRF.SystemFLemmasWeaken.
+Require Import SystemRF.Typing.
+Require Import SystemRF.LemmasWeakenWF.
+Require Import SystemRF.LemmasWellFormedness.
+Require Import SystemRF.LemmasTyping.
+Require Import SystemRF.LemmasWeakenTyp.
+Require Import SystemRF.LemmasSubtyping.
+Require Import SystemRF.SubstitutionLemmaTyp.
+Require Import SystemRF.LemmasNarrowing.
+Require Import SystemRF.LemmasTransitive. 
+
+Require Import ZArith.
+
+Lemma lem_list_compatM : forall (v:expr),
+  isList v -> isCompatM Length v.
+Proof. induction v; intros; simpl in H; try contradiction;
+  constructor; try apply IHv2; assumption. Qed.
+
+Lemma lem_invert_nil' : forall (g:env) (nl:expr) (t:type),
+  Hastype g nl t -> (forall (s : type) (qs : preds),
+    nl = Nil -> WFEnv g -> Subtype g t (TList s qs)
+             -> WFtype g (TList s qs) Star
+             -> exists s', Subtype g s' s /\ WFtype g s' Star /\
+                           isMono s' /\ noExists s' /\
+                  Subtype g (TList s' (PCons (eq (Ic 0) (length s' (BV 0))) PEmpty)) 
+                            (TList s  qs)).
+Proof. apply ( Hastype_ind
+    ( fun (g:env) (nl:expr) (t:type) => forall (s : type) (qs : preds),
+        nl = Nil -> WFEnv g -> Subtype g t (TList s qs)
+            -> WFtype g (TList s qs) Star
+            -> exists s', Subtype g s' s /\ WFtype g s' Star /\
+                          isMono s' /\ noExists s' /\
+                Subtype g (TList s' (PCons (eq (Ic 0) (length s' (BV 0))) PEmpty)) 
+                          (TList s  qs))
+  ); try discriminate; intros.
+  - (* isTNil *) inversion H4; subst g0 t1 p1 t2 p2.
+    exists t; repeat try split; destruct k;
+    try apply H1; try apply WFKind; trivial.
+  - (* isTSub *) apply H0; try apply lem_sub_trans with t Star k Star;
+    try (apply lem_typing_wf with e; assumption); assumption.
+  Qed.      
+
+Lemma lem_invert_nil : forall (g:env) (t:type) (ps:preds),
+    Hastype g Nil (TList t ps) 
+            -> WFEnv g -> WFtype g (TList t ps) Star
+            -> exists s', Subtype g s' t /\ WFtype g s' Star /\
+                          isMono s' /\ noExists s' /\
+                Subtype g (TList s' (PCons (eq (Ic 0) (length s' (BV 0))) PEmpty))
+                          (TList t ps).
+Proof. intros. apply lem_invert_nil' with Nil (TList t ps); 
+  try apply lem_sub_refl with Star; trivial.
+ Qed.      
+
+Lemma lem_invert_cons' : forall (g:env) (cns:expr) (t:type),
+  Hastype g cns t -> (forall (v1 v2: expr) (s : type) (qs : preds),
+    cns = Cons v1 v2 -> WFEnv g -> isValue v1 -> isValue v2
+            -> Subtype g t (TList s qs)
+            -> WFtype g (TList s qs) Star
+            -> exists s' ps, Subtype g s' s /\ WFtype g s' Star /\
+                             isMono s' /\ noExists s' /\
+                Hastype g v1 s' /\ Hastype g v2 (TList s' ps) /\
+                Subtype g 
+                  (TExists (TList s' ps)
+                      (TList s' (PCons (eq (App (Prim Succ) (length s' (BV 1))) 
+                                           (length s' (BV 0))) PEmpty))) 
+                  (TList s  qs)).
+Proof. apply ( Hastype_ind
+    ( fun (g:env) (cns:expr) (t:type) => forall (v1 v2: expr) (s : type) (qs : preds),
+    cns = Cons v1 v2 -> WFEnv g -> isValue v1 -> isValue v2
+            -> Subtype g t (TList s qs)
+            -> WFtype g (TList s qs) Star
+            -> exists s' ps, Subtype g s' s /\ WFtype g s' Star /\
+                             isMono s' /\ noExists s' /\
+                Hastype g v1 s' /\ Hastype g v2 (TList s' ps) /\
+                Subtype g 
+                  (TExists (TList s' ps)
+                      (TList s' (PCons (eq (App (Prim Succ) (length s' (BV 1))) 
+                                           (length s' (BV 0))) PEmpty))) 
+                  (TList s  qs))
+  ); try discriminate; intros .
+  - (* isTCons *) inversion H9; clear H2 H4; subst g0 t_x t0 t'.
+    apply lem_typing_wf in H1 as p_g_t; try apply H6;
+    apply lem_typing_wf in H3 as p_g_ltps; try apply H6;
+    apply lem_wftype_islct in p_g_ltps as Hlct;
+    unfold isLCT in Hlct; simpl in Hlct;
+    destruct Hlct as [Hlct Hlcp].    
+    pose proof lem_open_at_lc_at as [_ [Hopt Hopp]].
+    pose proof lem_subFV_notin as Hnot; 
+    destruct Hnot as [Hnot_e [Hnot_t _]].
+    pose proof lem_islc_at_weaken as [_ [Hwkt Hwkp]].
+    pose proof (fresh_var_not_elem nms g) as Hy;
+    set ( y:= fresh_var nms g) in Hy;
+    destruct Hy as [Hyn Hyg].
+    apply lem_free_bound_in_env with g t Star y 
+      in p_g_t as Hfr; try apply Hyg; 
+    destruct Hfr as [Hfr Hftv].
+    apply lem_free_bound_in_env with g (TList s qs) Star y 
+      in H10 as Hfr'; try apply Hyg; simpl in Hfr';
+    destruct Hfr' as [Hfr' Hftv']; 
+    apply not_elem_union_elim in Hfr'  as [Hfr'  _];
+    apply not_elem_union_elim in Hftv' as [Hftv' _];
+    apply H16 in Hyn as p_yg_lt_ls;
+    unfold unbindT in p_yg_lt_ls; simpl in p_yg_lt_ls;
+    rewrite Hopt with t 0 0 y in p_yg_lt_ls; 
+    rewrite Hopt with t 1 0 y in p_yg_lt_ls; 
+    try apply Hwkt with 0 0; try apply Hlct; auto.
+    inversion p_yg_lt_ls. subst g0 t1 p1 t2 p2.
+    injection H5 as H5'; subst eH eT;
+    exists t; exists ps; repeat try split; trivial;
+    try (rewrite <- Hnot_t with t y v2;
+         try rewrite <- Hnot_t with s y v2; trivial;
+         apply lem_subst_subtype_top with (TList t ps) Star Star);
+    try apply H13; try apply lem_weaken_wf_top; try apply p_g_t;
+    try apply lem_wflist_wftype with qs Star;
+    try apply wfenv_unique; trivial. 
+  - (* isTSub *) apply H0; 
+    try apply lem_sub_trans with t Star k Star;
+    try (apply lem_typing_wf with e; assumption); assumption.
+  Qed.      
+
+Lemma lem_invert_cons : forall (g:env) (v1 v2:expr) (t:type) (ps:preds),
+    Hastype g (Cons v1 v2) (TList t ps) 
+            -> WFEnv g -> isValue v1 -> isValue v2
+            -> WFtype g (TList t ps) Star
+            -> exists s' qs, Subtype g s' t /\ WFtype g s' Star /\
+                          isMono s' /\ noExists s' /\
+                Hastype g v1 s' /\ Hastype g v2 (TList s' qs) /\
+                Subtype g 
+                  (TExists (TList s' qs)
+                      (TList s' (PCons (eq (App (Prim Succ) (length s' (BV 1))) 
+                                           (length s' (BV 0))) PEmpty))) 
+                  (TList t ps).
+Proof. intros. apply lem_invert_cons' with (Cons v1 v2) (TList t ps); 
+  try apply lem_sub_refl with Star; trivial.
+ Qed.     
+
+Lemma lem_invert_tlist' : forall (g:env) (ce:expr) (t:type),
+  Hastype g ce t -> (forall (v1 v2 : expr) (s : type) (qs : preds),
+    ce = Cons v1 v2 -> isValue v2
+                    -> WFEnv g -> Subtype g t (TList s qs)
+                    -> WFtype g (TList s qs) Star
+                    -> exists (rs : preds), Hastype g v1 s /\
+                        Hastype g v2 (TList s rs)).
+Proof. apply ( Hastype_ind
+    ( fun (g:env) (ce:expr) (t:type) 
+      => forall (v1 v2 : expr) (s : type) (qs : preds),
+            ce = Cons v1 v2 -> isValue v2
+                    -> WFEnv g -> Subtype g t (TList s qs)
+                    -> WFtype g (TList s qs) Star
+                    -> exists (rs : preds), Hastype g v1 s /\
+                        Hastype g v2 (TList s rs))
+  ); try discriminate; intros.  
+  - (* isTCons *) injection H5 as Hv1 Hv2; subst eH eT.
+    apply lem_typing_wf in H1 as p_g_t;
+    try apply lem_wftype_islct in p_g_t as Hlct;
+    pose proof lem_open_at_lc_at as [_ [H' _]];
+    pose proof lem_subFV_notin as [_ [Hsub _]]; trivial.
+    inversion H8.
+    set (y := fresh_var nms g); pose proof (fresh_var_not_elem nms g);
+    destruct H15.
+    apply (H14 y) in H15 as p_yg_sub; unfold unbindT in p_yg_sub; 
+    simpl in p_yg_sub; inversion p_yg_sub.
+    rewrite H' with t 0 0 y in H21; auto.
+    apply lem_subst_subtype_top
+      with g y v2 (TList t ps) t s Star Star in H21;
+    try rewrite Hsub in H21; try rewrite Hsub in H21;
+    try exists ps; try split; try apply H3;
+    try match goal with
+        | [ |- Hastype _ v1 _] => apply TSub with t Star
+        | [ |- Hastype _ v2 _] => apply TSub with (TList t ps) Star
+        end;
+    try apply SList with nms; intros; try apply IRefl;
+    try apply lem_typing_wf in H3 as p_g_tps;
+    try apply lem_free_bound_in_env with g Star;
+    apply lem_wflist_wftype in H9 as p_g_s; trivial;
+    try apply lem_weaken_wf_top;
+    try apply wfenv_unique; trivial.
+    inversion p_g_tps; try inversion H24;
+    try apply WFList with Star;
+    try apply WFListR with nms1; try apply WFList with Star;
+    try rewrite <- lem_erase_subtype with g t s;
+    trivial.
+  - (* TSub *) apply H0 with qs;
+    try apply lem_sub_trans with t Star k Star;
+    try apply lem_typing_wf in H; trivial.
+  Qed.
+    
+Lemma lem_invert_tlist : forall (g:env) (v1 v2:expr) (t:type) (ps:preds),
+    Hastype g (Cons v1 v2) (TList t ps) 
+                  -> WFEnv g -> WFtype g (TList t ps) Star
+                  -> isValue v1 -> isValue v2
+                  -> exists qs:preds, Hastype g v1 t /\
+                        Hastype g v2 (TList t qs).
+Proof. intros; inversion H.
+  apply lem_invert_tlist' with (Cons v1 v2) s ps; trivial.
+ Qed.      
+
+Lemma lem_list_eq_length: forall (g:env) (v:expr) (s:type) (rs:preds),
+    Hastype g v (TList s rs) -> WFEnv g 
+            -> isList v -> isValue v
+            -> isMono s -> noExists s
+            -> Hastype g v 
+                       (TList s (PCons (eq (length s v)
+                                           (length s (BV 0))) rs)). 
+Proof. intros g; induction v; intros;
+  simpl in H1; try contradiction;
+  assert (WFtype g s Star) as p_g_s 
+      by (apply lem_wflist_wftype with rs Star; 
+          try apply lem_typing_wf with (Cons v1 v2);
+          try apply lem_typing_wf with Nil;   trivial);
+  apply lem_typing_hasftype in H as p_v_ers; try apply H0;
+  apply lem_wftype_islct in p_g_s as Hlcs;
+  pose proof lem_open_at_lc_at as [Hope [Hopt _]];
+  pose proof lem_islc_at_weaken as [Hwke [Hwkt _]];
+  pose proof lem_subFV_notin as Hnot; 
+  destruct Hnot as [Hnot_e [Hnot_t Hnot_p]].
+  - (* Nil *) pose proof TNil.
+    assert (isCompatM Length Nil) as pf
+      by constructor.
+    assert (Some (deltaM Length Nil pf) 
+              = Some (Ic 0)) 
+      as delM by (rewrite deltaM_deltaM'; simpl; reflexivity).
+    injection delM as delM.
+    apply lem_invert_nil in H as Hinv;
+    try apply lem_typing_wf with Nil; trivial.
+    destruct Hinv as [s' [p_s'_s [p_g_s' [mono [noex p_g_ls'_ls]]]]].
+    inversion p_g_ls'_ls; subst g0 t1 p1 t2 p2;
+    apply lem_wftype_islct in p_g_s' as Hlcs';
+    apply TSub with 
+      (TList s' (PCons (eq (Ic 0) (length s' (BV 0))) PEmpty)) Star;
+    try apply TNil with Star; 
+    try apply lem_wflist_eq_length; trivial;
+    try apply lem_typing_wf with Nil; trivial.
+    
+    apply SList with (union nms (binds g)); trivial; intros;
+    apply not_elem_union_elim in H6; destruct H6;
+    assert (
+        unbindP y (PCons (eq (length s Nil) 
+                             (length s (BV 0))) rs)
+            = strengthen 
+                (unbindP y (PCons (eq (length s Nil) 
+                                      (length s (BV 0))) PEmpty)) 
+                (unbindP y rs) )
+        as Hpred by reflexivity. rewrite Hpred.
+    apply IConj;
+    unfold unbindP; simpl;
+    try rewrite Hopt with s' 0 0 y;
+    try rewrite Hopt with s  0 0 y; trivial.
+
+    (* 1 *)
+    apply ITrans with 
+      (PCons (App (App (Prim Eq) (Ic 0)) 
+                  (App (AppT (Prim Length) s) (FV y))) PEmpty);
+    try apply ILenSub;
+    try apply lem_weaken_subtype_top with Star Star;
+    try apply IEvals2; try apply lem_step_evals;
+    try apply EApp1; try apply EApp2; try apply val_Prm;
+    try rewrite <- delM; try apply EPrimM;
+    try apply wfenv_unique; trivial.
+    
+    (* 2 *)
+    apply H12 in H6 as Himpl;
+    unfold unbindP in Himpl; simpl in Himpl;
+    try rewrite Hopt with s' 0 0 y in Himpl;
+    try apply Himpl; trivial.
+  - (* TCons *)
+    assert (isList (Cons v1 v2)) as Hv by (simpl; trivial).
+    assert (isCompatM Length (Cons v1 v2)) as pf
+      by (apply lem_list_compatM; assumption).
+    inversion pf as [pf'|eH' eT' pf' HeH' HeT'];
+      subst eH' eT'; clear HeH'.
+    inversion H2; subst v0 v3.
+    assert (Some (deltaM Length (Cons v1 v2) pf) 
+              = Some (App (Prim Succ) (deltaM Length v2 pf'))) 
+      as delM by (rewrite deltaM_deltaM'; simpl;
+                  rewrite <- deltaM_deltaM' with Length v2 pf';
+                  reflexivity).
+    injection delM as delM.
+    
+    apply lem_invert_cons in H as Hinv;
+    try apply lem_typing_wf with (Cons v1 v2); trivial;
+    destruct Hinv as [s' [qs [p_s'_s [p_g_s' 
+        [mono [noex [p_e1_s' [p_e2_ls' p_g_ls'_ls]]]]]]]].
+    inversion p_g_ls'_ls; subst g0 t_x t t'.
+
+    apply lem_typing_hasftype in p_e2_ls' as p_e2_erls'; try apply H0;
+    apply lem_wftype_islct in p_g_s' as Hlcs'.
+
+    apply TSub with     (* second subtyping obligation *)
+      (TList s' (PCons (eq (App (Prim Succ) (length s' v2)) 
+                           (length s' (BV 0))) PEmpty)) Star;
+    try apply TSub with  (* first subtyping obligation *)
+      (TExists (TList s' (PCons (eq (length s' v2) (length s' (BV 0))) qs))
+        (TList s' (PCons (eq (App (Prim Succ) (length s' (BV 1))) 
+                             (length s' (BV 0))) PEmpty))) Star;
+    try apply TCons; try apply IHv2;
+    trivial;
+
+    apply lem_typing_wf in H as p_g_ls;
+    apply lem_typing_wf in p_e2_ls' as p_g_ls';
+    try apply lem_typ_islc in p_e1_s' as Hlcv1;
+    try apply lem_typ_islc in p_e2_ls' as Hlcv2;    
+    try apply lem_wflist_eq_succ_length; 
+    try apply lem_wflist_eq_length; 
+    try apply WFList with Star; auto.
+
+    (* prove first subtyping obligation *)
+    try apply SBind with (binds g); intros;
+    try assert (y =? y = true) 
+      as Hyeq by (apply Nat.eqb_eq; reflexivity);
+    unfold unbindT; simpl;
+    try rewrite Hopt with s'  0 0 y;
+    try rewrite Hopt with s'  1 0 y;
+    unfold isLCT; simpl; try repeat split;
+    try apply Hwke with 0 0;
+    try apply Hwkt with 0 0; auto;
+    try apply SList with (names_add y (binds g));
+    try apply lem_sub_refl with Star;
+    try (apply lem_weaken_wf_top; apply p_g_s' || apply H5);
+    intros; try apply not_elem_names_add_elim in H6; try destruct H6;
+    try assert (y =? y0 = false) 
+      as Hnyeq by (apply Nat.eqb_neq; symmetry; trivial);
+    unfold unbindP; simpl;
+    try rewrite Hope with v2 0 0 y0;
+    try rewrite Hopt with s'  0 0 y0; trivial.
+
+    try assert (
+        PCons (App (App (Prim Eq) (App (Prim Succ) (App (AppT (Prim Length) s') v2))) 
+                   (App (AppT (Prim Length) s') (FV y0))) PEmpty
+      = (psubFV y v2
+          (PCons (App (App (Prim Eq) (App (Prim Succ) (App (AppT (Prim Length) s') (FV y)))) 
+                      (App (AppT (Prim Length) s') (FV y0))) PEmpty))
+    ) as Htyp by (unfold psubFV; simpl; fold tsubFV;
+                  rewrite Hnyeq; rewrite Hyeq; rewrite Hnot_t;
+                  try apply lem_free_bound_in_env with g Star; trivial);
+    try rewrite Htyp;
+    try apply IExactLen with s' qs;
+    try apply lem_weaken_wf_top; try apply lem_weaken_wf_top;
+    try apply not_elem_names_add_intro;
+    simpl; intuition;
+
+    try repeat apply lem_weaken_typ_top;
+    try apply TSub with (TList t ps) Star;
+    try apply SList with empty; intros; try apply IFaith; 
+    try apply WFEBind with Star;
+    try repeat apply lem_weaken_wf_top;
+
+    unfold unique; simpl; try repeat split; fold unique;
+    try apply not_elem_names_add_intro; try repeat split;
+    try apply lem_wflist_eq_length;
+    try (apply wfenv_unique; apply H0); auto. 
+
+    pose proof (fresh_var_not_elem nms g);
+    set (y0 := fresh_var nms g) in H5; destruct H5;
+    apply H12 in H5 as p_yg_ls'_ls;
+    unfold unbindT in p_yg_ls'_ls; simpl in p_yg_ls'_ls;
+    try rewrite Hopt with s' 0 0 y0 in p_yg_ls'_ls;
+    try rewrite Hopt with s' 1 0 y0 in p_yg_ls'_ls; 
+    try apply Hwkt with 0 0; auto.
+    inversion p_yg_ls'_ls; subst g0 t1 p1 t2 p2.
+
+    apply SList with (names_add y0 (union (union nms nms0) (binds g))); 
+    trivial; intros;
+    apply not_elem_names_add_elim in H9; destruct H9.
+    apply not_elem_union_elim in H11; destruct H11;
+    apply not_elem_union_elim in H11; destruct H11;
+    assert (
+        unbindP y (PCons (eq (length s (Cons v1 v2)) 
+                             (length s (BV 0))) rs)
+            = strengthen 
+                (unbindP y (PCons (eq (length s (Cons v1 v2)) 
+                                      (length s (BV 0))) PEmpty)) 
+                (unbindP y rs) )
+        as Hpred by reflexivity. rewrite Hpred.
+    apply IConj;
+    unfold unbindP; simpl;
+    try rewrite Hope with v1 0 0 y;
+    try rewrite Hope with v2 0 0 y;
+    try rewrite Hopt with s' 0 0 y;
+    try rewrite Hopt with s  0 0 y; trivial.
+
+    (* 1:  Implies (ECons y (TList s' PEmpty) g) 
+        (PCons (App (App (Prim Eq) (App (Prim Succ) (App (AppT (Prim Length) s') v2))) 
+                                    (App (AppT (Prim Length) s') (FV y))) PEmpty) 
+        (PCons (App (App (Prim Eq) (App (AppT (Prim Length) s) (Cons v1 v2))) 
+                                    (App (AppT (Prim Length) s) (FV y))) PEmpty) *)
+    apply ITrans with 
+        (PCons (App (App (Prim Eq) (App (Prim Succ) (App (AppT (Prim Length) s) v2)))
+                    (App (AppT (Prim Length) s) (FV y))) PEmpty);
+    try apply ILenSub2;
+    try apply lem_weaken_subtype_top with Star Star; 
+    
+    try apply ITrans with 
+        (PCons (App (App (Prim Eq) (App (Prim Succ) (deltaM Length v2 pf'))) 
+                    (App (AppT (Prim Length) s) (FV y))) PEmpty);
+    try ( apply IEvals; apply lem_step_evals; 
+          apply EApp1; apply EApp2; try apply EApp2;
+          try apply val_Prm; trivial; apply EPrimM);
+    try ( apply IEvals2; apply lem_step_evals; 
+          apply EApp1; apply EApp2; try apply val_Prm;
+          try apply EPrimM; rewrite <- delM; apply EPrimM);
+    try apply wfenv_unique; trivial.
+    
+    (* 2:  Implies (ECons y (TList s' PEmpty) g) 
+        (PCons (App (App (Prim Eq) (App (Prim Succ) (App (AppT (Prim Length) s') v2))) 
+                                    (App (AppT (Prim Length) s') (FV y))) PEmpty) 
+        (openP_at 0 y rs)
+    
+    *)
+    apply H17 in H14 as Himpl; 
+    unfold unbindP in Himpl; simpl in Himpl;
+    try rewrite Hopt with s' 0 0 y  in Himpl;
+    try apply Himpl; trivial.
+
+    assert (ECons y (TList s' PEmpty) (ECons y0 (TList s' qs) g)
+            = concatE (ECons y0 (TList s' qs) g) 
+                      (ECons y (TList s' PEmpty) Empty)
+    ) as Henv by reflexivity; rewrite Henv in Himpl.
+    apply ISub 
+      with g (ECons y (TList s' PEmpty) Empty) y0 v2 (TList s' qs)
+           (PCons (App (App (Prim Eq) (App (Prim Succ) (App (AppT (Prim Length) s') (FV y0)))) 
+                       (App (AppT (Prim Length) s') (FV y))) PEmpty) 
+           (openP_at 0 y rs)
+      in Himpl; simpl in Himpl;
+    try assert (y0 =? y0 = true) 
+      as Hy0eq by (apply Nat.eqb_eq; reflexivity);
+    try assert (y0 =? y = false) 
+      as Hnyeq by (apply Nat.eqb_neq; symmetry; trivial);
+    simpl in Hy0eq;  simpl in Hnyeq;
+    try rewrite Hy0eq in Himpl;
+    try rewrite Hnyeq in Himpl; clear Henv Hy0eq Hnyeq;
+    try rewrite lem_commute_psubFV_unbindP in Himpl;
+    try rewrite Hnot_p in Himpl;
+    try rewrite Hnot_t in Himpl; try apply Himpl;
+    
+    try apply lem_free_bound_in_env with g Star;
+    apply lem_free_bound_in_env with g (TList s rs) Star y0 
+        in p_g_ls as Hfree; try simpl in Hfree;
+    try destruct Hfree as [Hfree _];
+    try apply not_elem_union_elim in Hfree as [_ Hfree];
+    pose proof fv_open_at_elim as [_ [_ Hfvop]];
+
+    try apply intersect_names_add_intro_r;
+    try apply intersect_empty_r;
+    try apply not_elem_names_add_intro;
+    try (apply not_elem_subset with (names_add y (fvP rs));
+         apply Hfvop || apply not_elem_names_add_intro);
+    simpl; try split; try apply wfenv_unique; auto.
+  Qed.
+
+Lemma lem_list_subtype_conj : 
+  forall (g:env) (s:type) (ps:preds) (t:type) (q:expr) (qs:preds),
+         Subtype g (TList s ps) (TList t (PCons q PEmpty))
+      -> Subtype g (TList s ps) (TList t qs)
+      -> Subtype g (TList s ps) (TList t (PCons q qs)).
+Proof. intros. inversion H; subst g0 t1 p1 t2 p2;
+  inversion H0; subst g0 t1 p1 t2 p2.
+  apply SList with (union nms nms0); try apply H5;
+  intros; unfold unbindP; simpl;
+  assert (
+    PCons (open_at 0 y q) (openP_at 0 y qs)
+      = strengthen (PCons (open_at 0 y q) PEmpty) (openP_at 0 y qs)
+    ) as Hqqs by reflexivity; rewrite Hqqs; 
+  apply IConj; apply H7 || apply H9;
+  apply not_elem_union_elim in H1; destruct H1; trivial.
+  Qed.
